Added serialisation and merkleisation for Uint16
Removed Uint8 type as it is not used

src/dafny/ssz/IntSeDes.dfy
@@ -1,9 +1,9 @@
 /*
  * Copyright 2020 ConsenSys AG.
  *
- * Licensed under the Apache License, Version 2.0 (the "License"); you may 
+ * Licensed under the Apache License, Version 2.n (the "License"); you may 
  * not use this file except in compliance with the License. You may obtain 
- * a copy of the License at http://www.apache.org/licenses/LICENSE-2.0
+ * a copy of the License at http://www.apache.org/licenses/LICENSE-2.n
  *
  * Unless required by applicable law or agreed to in writing, software dis-
  * tributed under the License is distributed on an "AS IS" BASIS, WITHOUT 
@@ -13,7 +13,10 @@
  */
 
 include "../utils/NativeTypes.dfy"
+include "../utils/NonNativeTypes.dfy"
 include "../utils/Eth2Types.dfy"
+include "../utils/MathHelpers.dfy"
+include "../libraries/integers/power.i.dfy"
 
 /**
  *  Integers serialisation, desrialisation.
@@ -22,26 +25,82 @@ include "../utils/Eth2Types.dfy"
 module IntSeDes {
 
     import opened NativeTypes
+    import opened NonNativeTypes
     import opened Eth2Types
+    import opened MathHelpers
+    import opened Math__power_i
+    import opened Math__power_s
 
     //  Uintk serialisation and deserielisation.
-
-    /** Uint8. */
-    function method uint8ToBytes(n: uint8) : seq<byte> 
-        ensures |uint8ToBytes(n)| == 1
+      
+    /**
+     * Computes the little endian serialisation of a natural value
+     *
+     * @param n        The value to serialise
+     * @param length   Length of the serialisation.
+     * @requires       n < power(0x100,length) 
+     *
+     * @returns        The `length`-byte little endian serialisation of `n`
+     *
+     */
+    function method int_to_bytes(n: nat, length: nat) : bytes
+    requires n as nat < power(0x100, length)
+    ensures |int_to_bytes(n,length)| == length as int
     {
-        [n as byte]
-    }
- 
-    function method byteToUint8(b: byte) : uint8
-    {
-        (b as uint8)
+        reveal_power();
+        if(length == 0) then
+            []
+        else
+            [(n % 0x100) as uint8] +
+            int_to_bytes(n / 0x100, length-1)
     }
 
-    /** Encode/decode Uint8 yields Identity. */
-    lemma uint8AsBytesInvolutive(n : uint8) 
-        ensures byteToUint8(uint8ToBytes(n)[0]) == n
-    {   //  Thanks Dafny
+    /**
+     * Deserialise a sequence of bytes to a natural number using little endian
+     * interpretation
+     *
+     * @param s Sequence of bytes. Must be no longer than 8 bytes.
+     *
+     * @returns The natural value corresponding to the little endian
+     * deserialisation of `s`
+     */
+    function method bytes_to_int(s: bytes):nat
+    ensures bytes_to_int(s)  < power(0x100, |s|)
+    {
+        reveal_power();
+        if(|s| == 0) then
+            0
+        else
+            s[0] as nat + bytes_to_int(s[1..])*0x100
     }
+
+    /** `bytes_to_int` is the inverse of `int_to_bytes` */
+    lemma lemmaBytesToIntIsTheInverseOfIntToBytes(n: nat, length: nat)
+    requires int_to_bytes.requires(n,length)
+    ensures bytes_to_int(int_to_bytes(n,length)) == n 
+    { // Thanks Dafny
+    }
+
+    /** `int_to_bytes` is the inverse of `bytes_to_int` */
+    lemma lemmaIntToBytesIsTheInverseOfBytesToInt(s: bytes)
+    requires bytes_to_int.requires(s)
+    ensures int_to_bytes(bytes_to_int(s),|s|) == s 
+    { 
+        if(|s|==0)
+        {
+            // Thanks Dafny
+        }
+        else
+        {
+            calc == {
+                int_to_bytes(bytes_to_int(s),|s|);
+                int_to_bytes(s[0] as nat + bytes_to_int(s[1..])*0x100,|s|);
+                [s[0]] + int_to_bytes(bytes_to_int(s[1..]),(|s|-1));
+                // via induction
+                [s[0]] + s[1..];
+                s;
+            }
+        }
+    }     
 
 }
